\input{header.tex}
\setcounter{theorem}{0}
\begin{exercise} BH.8.1
\begin{solution}
Here are two ways, one a bit cumbersome, but straightforward, the second with Theorem 8.1.1.

$Y=g(X) = e^{-X}$, hence $g(x) = e^{-x}$. Note that $g(x) \in (0, 1]$ for $x\geq 0$. Also, $g^{-1}(x) = -\log x$. And so,
\begin{align*}
  \P{Y\leq y} &\stackrel1= \P{X \geq g^{-1}(y)} = \P{X \geq -\log y} = \P{X\geq \log 1/y} = e^{-\log 1/y} =  y.
\end{align*}
To understand step 1 in which we flip the inequality sign, make a drawing of $e^{-x}$ and note that it decreases.
For the PDF, take the derivative with respect to $y$.

Now the other method. Use the mnemonic $f_{x}(x) \d x = f_{Y}(y) \d y$. Divide both sides by $\d y$ and take the absolute value:
\begin{align*}
  f_{Y}(y) = f_{X}(x) |\frac{\d x}{\d y}|.
\end{align*}
Now, $\d y/\d x = \d g/\d x = -e^{-x}$. Hence,
\begin{align*}
  f_{Y}(y) = f_{X}(x) |\frac{\d x}{\d y}| = e^{-x} \frac{1}{e^{-x}} \1 {0< y \leq 1},
\end{align*}
where we include the support of $Y$ in the last step.

\end{solution}
\end{exercise}
\input{trailer.tex}
